SciLean/Tactic/MathlibCompiledTactics.lean
@@ -1,5 +1,4 @@
 import Mathlib.Tactic.FunProp
 import Mathlib.Tactic.FunTrans.Elab
 import Mathlib.Tactic.FunTrans.Attr
-import SciLean.Tactic.LSimp.Elab
 import SciLean.Tactic.LSimp.Main
