test/lsimp_basic_tests.lean
@@ -5,150 +5,320 @@ import SciLean.Tactic.MathlibCompiledTactics
 import SciLean.Util.Profile
 
 
--- example (n : Nat) :
---   n
---   =
---   n := by (conv => lhs; lsimp)
+example (n : Nat) :
+  n
+  =
+  n := by (conv => lhs; lsimp)
 
--- example (n : Nat) :
---   (let a := 1; a + n)
---   =
---   (1 + n) := by (conv => lhs; lsimp)
+example (n : Nat) :
+  (let a := 1; a + n)
+  =
+  (1 + n) := by (conv => lhs; lsimp)
 
--- example (n : Nat) :
---   (0 + n)
---   =
---   n := by (conv => lhs; lsimp)
+example (n : Nat) :
+  (0 + n)
+  =
+  n := by (conv => lhs; lsimp)
 
--- example (n : Nat) :
---   (0 + 1 * n)
---   =
---   n := by (conv => lhs; lsimp)
+example (n : Nat) :
+  (0 + 1 * n)
+  =
+  n := by (conv => lhs; lsimp)
 
--- example (n : Nat) :
---   (let a := (0 + 1 * n); a)
---   =
---   n := by (conv => lhs; lsimp)
+example (n : Nat) :
+  (let a := (0 + 1 * n); a)
+  =
+  n := by (conv => lhs; lsimp)
 
--- example (n : Nat) :
---     (let a :=
---        let c := 0 + n
---        let d := c + 0 + 3
---        c + d + 1 * n + 2
---      let b := a + 5
---      a + b)
---     =
---     n + (n + 3) + n + 2 + (n + (n + 3) + n + 2 + 5) := by
---   (conv => lhs; lsimp)
+example (n : Nat) :
+    (let a :=
+       let c := 0 + n
+       let d := c + 0 + 3
+       c + d + 1 * n + 2
+     let b := a + 5
+     a + b)
+    =
+    n + (n + 3) + n + 2 + (n + (n + 3) + n + 2 + 5) := by
+  (conv => lhs; lsimp)
 
--- example (n : Nat) (i : Fin n) :
---     (let j := 2*i.1
---      let hj : j < 2*n := by omega
---      let j : Fin (2*n) := ⟨j, hj⟩
---      let k :=
---        let a := j + j
---        a + j
---      j + k)
---     =
---     let j := 2*i.1
---     let hj : j < 2*n := by omega
---     let j : Fin (2*n) := ⟨j, hj⟩
---     (j + (j + j + j)) := by
---   (conv => lhs; lsimp)
+example (n : Nat) (i : Fin n) :
+    (let j := 2*i.1
+     let hj : j < 2*n := by omega
+     let j : Fin (2*n) := ⟨j, hj⟩
+     let k :=
+       let a := j + j
+       a + j
+     j + k)
+    =
+    let j := 2*i.1
+    let hj : j < 2*n := by omega
+    let j : Fin (2*n) := ⟨j, hj⟩
+    (j + (j + j + j)) := by
+  (conv => lhs; lsimp)
 
--- -- tests under lambda binder
+-- tests under lambda binder
 
--- example :
---   (fun n : Nat => n)
---   =
---   (fun n : Nat => n) := by (conv => lhs; lsimp)
+example :
+  (fun n : Nat => n)
+  =
+  (fun n : Nat => n) := by (conv => lhs; lsimp)
 
--- example :
---   (fun n => let a := 1; a + n)
---   =
---   (fun n => 1 + n) := by (conv => lhs; lsimp)
-
-
--- example :
---   (fun n => let a := (0 + 1 * n * 1 * 2); a)
---   =
---   (fun n => n * 2) := by (conv => lhs; lsimp)
+example :
+  (fun n => let a := 1; a + n)
+  =
+  (fun n => 1 + n) := by (conv => lhs; lsimp)
 
 
--- example :
---     (fun n : Nat=>
---      let c := n
---      let a := c + 1 * n
---      a)
---     =
---     (fun n => n + n) := by
---   (conv => lhs; lsimp)
+example :
+  (fun n => let a := (0 + 1 * n * 1 * 2); a)
+  =
+  (fun n => n * 2) := by (conv => lhs; lsimp)
 
 
--- example :
---     (fun (n : Nat) (i : Fin n) =>
---      let j := 2*i.1
---      let hj : j < 2*n := by omega
---      let j : Fin (2*n) := ⟨j, hj⟩
---      let k :=
---        let a := j + j
---        a + j
---      j + k)
---     =
---     fun (n : Nat) (i : Fin n) =>
---     let j := 2*i.1
---     let hj : j < 2*n := by omega
---     let j : Fin (2*n) := ⟨j, hj⟩
---     (j + (j + j + j)) := by
---   (conv => lhs; lsimp)
+example :
+    (fun n : Nat=>
+     let c := n
+     let a := c + 1 * n
+     a)
+    =
+    (fun n => n + n) := by
+  (conv => lhs; lsimp)
 
 
+example :
+    (fun (n : Nat) (i : Fin n) =>
+     let j := 2*i.1
+     let hj : j < 2*n := by omega
+     let j : Fin (2*n) := ⟨j, hj⟩
+     let k :=
+       let a := j + j
+       a + j
+     j + k)
+    =
+    fun (n : Nat) (i : Fin n) =>
+    let j := 2*i.1
+    let hj : j < 2*n := by omega
+    let j : Fin (2*n) := ⟨j, hj⟩
+    (j + (j + j + j)) := by
+  (conv => lhs; lsimp)
 
 
 
--- set_default_scalar Float
-
--- open SciLean
-
--- -- set_option trace.Meta.Tactic.simp.proj true
--- set_option trace.Meta.Tactic.simp.steps true
-
-
--- #check (∇ x : Float, let y := x * x; x * y)
---   rewrite_by
---     unfold scalarGradient
---     lsimp
-
-
--- #check (∂ x : Float, let y := x * x; x * y)
---   rewrite_by
---     unfold scalarCDeriv
---     lsimp
-
-
--- #check (∂> x : Float, let y := x * x; x * y)
---   rewrite_by
---     lsimp
-
-
--- #check Nat
-
--- #check (∂> x : Float, let y := x * x; let z := x * y; x * y * z)
---   rewrite_by
---     lsimp
-
-set_option profiler true
-
-set_option trace.Meta.Tactic.simp.steps true
 
 set_default_scalar Float
 
 open SciLean
 
+-- set_option trace.Meta.Tactic.simp.numSteps true
+-- set_option trace.Meta.Tactic.simp.time true
+
+
+-- -- set_option trace.Meta.Tactic.simp.proj true
+-- set_option trace.Meta.Tactic.simp.steps true
+
+
+open Lean Meta Elab Term Tactic Conv in
+elab "timeTactic" t:conv : conv => do
+
+  let target ← getMainTarget
+  let ((targetNew, proof),time) ← Aesop.time <| convert target (withTacticInfoContext (← getRef) (evalTactic t))
+  liftMetaTactic1 fun mvarId => mvarId.replaceTargetEq targetNew proof
+  IO.println s!"tactic {t.raw.prettyPrint} took {time.printAsMillis}"
+
+
+
+#check (∇ x : Float, let y := x * x; x * y)
+  rewrite_by
+    unfold scalarGradient
+    lsimp
+
+
+-- set_option trace.Meta.Tactic.fun_trans true in
+
+-- #check (∇ (x : Float×Float), let y := x + x; let z := x + y; y.1*z.2)
+--   rewrite_by
+--     unfold scalarGradient
+--     timeTactic autodiff
+
+-- #check (∇ (x : Float×Float), let y := x + x; let z := x + y; y.1*z.2)
+--   rewrite_by
+--     unfold scalarGradient
+--     timeTactic lsimp
+
+#check (∇ x : Float,
+          let x1 := x * x
+          let x2 := x * x1
+          let x3 := x * x2
+          let x4 := x * x3
+          let x5 := x * x4
+          let x6 := x * x5
+          -- let x8 := x * x7
+          -- let x9 := x * x8
+          -- let x10 := x * x9
+          -- let x11 := x * x10
+          x6)
+  rewrite_by
+    unfold scalarGradient
+    lsimp
+
+
+#exit
+
+#check (∂ x : Float, let y := x * x; x * y)
+  rewrite_by
+    unfold scalarCDeriv
+    lsimp
+
+
+#check (∂> x : Float, let y := x * x; x * y)
+  rewrite_by
+    lsimp
+
+
+-- #check Nat
+
+#check (∂> x : Float, let y := x * x; let z := x * y; x * y * z)
+  rewrite_by
+    lsimp
+
+set_option profiler true
+
+set_option trace.Meta.Tactic.simp.numSteps true
+set_option trace.Meta.Tactic.simp.time true
+-- set_option trace.Meta.Tactic.simp.proj true
+-- set_option trace.Meta.Tactic.simp.heads true
+-- set_option trace.Meta.Tactic.simp.cache true
+
+set_default_scalar Float
+
+open SciLean
+
+
+#check (structProj 1 ())
+  rewrite_by
+    unfold scalarGradient
+    lsimp
+    lsimp
+
+
+
+-- #check (∇ x : Float, let y := x * x; let z := x * y; x * y * z)
+--   rewrite_by
+--     unfold scalarGradient
+--     lsimp
+--     lsimp-- 16107 steps & 4.45s | with cache: 1295 steps && 709ms
+
+
 -- #check (∇ x : Float, let y := x * x; let z := x * y; x * y * z)
 --   rewrite_by
 --     unfold scalarGradient
 --     lsimp -- 16107 steps & 4.45s | with cache: 1295 steps && 709ms
+
+
+#check (∇ x : Float,
+          let x1 := x * x
+          let x2 := x1 * x1
+          let x3 := x2 * x2
+          let x4 := x3 * x3
+          let x5 := x4 * x4
+          let x6 := x5 * x5
+          -- let x8 := x * x7
+          -- let x9 := x * x8
+          -- let x10 := x * x9
+          -- let x11 := x * x10
+          x6)
+  rewrite_by
+    unfold scalarGradient
+    lsimp
+
+
+
+
+#check (∇ x : Float,
+          let x1 := x * x
+          let x2 := x * x1
+          let x3 := x * x2
+          let x4 := x * x3
+          let x5 := x * x4
+          let x6 := x * x5
+          -- let x8 := x * x7
+          -- let x9 := x * x8
+          -- let x10 := x * x9
+          -- let x11 := x * x10
+          x6)
+  rewrite_by
+    unfold scalarGradient
+    lsimp
+
+
+
+#check (∇ x : Float,
+          let x1 := x * x
+          let x2 := x * x1
+          let x3 := x * x2
+          let x4 := x * x3
+          let x5 := x * x4
+          let x6 := x * x5
+          -- let x8 := x * x7
+          -- let x9 := x * x8
+          -- let x10 := x * x9
+          -- let x11 := x * x10
+          x6)
+  rewrite_by
+    unfold scalarGradient
+    lsimp
+
+
+
+
+-- #check (∂> x : Float,
+--           let x1 := x * x
+--           let x2 := x * x1
+--           let x3 := x * x2
+--           let x4 := x * x3
+--           let x5 := x * x4
+--           let x6 := x * x5
+--           let x7 := x * x6
+--           let x8 := x * x7
+--           let x9 := x * x8
+--           let x10 := x * x9
+--           let x11 := x * x10
+--           x10 * x11)
+--   rewrite_by
+--     unfold scalarGradient
+--     lsimp
+
+
+
+
+
+#exit
+
+
+#check (∇ x : Float,
+          let x1 := x * x
+          let x2 := x * x1
+          let x3 := x * x2
+          let x4 := x * x3
+          x3 * x4)
+  rewrite_by
+    unfold scalarGradient
+    lsimp
+    simp
+
+
+#exit
+
+#check (∇ x : Float,
+          let x1 := x * x
+          let x2 := x * x1
+          let x3 := x * x2
+          let x4 := x * x3
+          let x5 := x * x4
+          x * x1 * x2 * x3 * x4 * x5)
+  rewrite_by
+    unfold scalarGradient
+    lsimp
 
 
 
@@ -161,17 +331,4 @@ open SciLean
           x * x1 * x2 * x3 * x4 * x5)
   rewrite_by
     unfold scalarGradient
-    lsimp -- 16107 steps & 4.45s | with cache: 1295 steps && 709ms
-
-
-
--- #check (∇ x : Float,
---           let x1 := x * x
---           let x2 := x * x1
---           let x3 := x * x2
---           let x4 := x * x3
---           let x5 := x * x4
---           x * x1 * x2 * x3 * x4 * x5)
---   rewrite_by
---     unfold scalarGradient
---     autodiff
+    autodiff
